src/verit/veritParser.mly
@@ -41,8 +41,8 @@
 %token EOL SAT
 %token COLON
 %token LPAR RPAR LBRACKET RBRACKET
-%token NOT XOR ITE EQ LT LEQ GT GEQ PLUS MINUS MULT OPP LET DIST BBT BITOF BVAND BVOR
-%token INPU DEEP TRUE FALS ANDP ANDN ORP ORN XORP1 XORP2 XORN1 XORN2 IMPP IMPN1 IMPN2 EQUP1 EQUP2 EQUN1 EQUN2 ITEP1 ITEP2 ITEN1 ITEN2 EQRE EQTR EQCO EQCP DLGE LAGE LATA DLDE LADE FINS EINS SKEA SKAA QNTS QNTM RESO WEAK AND NOR OR NAND XOR1 XOR2 NXOR1 NXOR2 IMP NIMP1 NIMP2 EQU1 EQU2 NEQU1 NEQU2 ITE1 ITE2 NITE1 NITE2 TPAL TLAP TPLE TPNE TPDE TPSA TPIE TPMA TPBR TPBE TPSC TPPP TPQT TPQS TPSK SUBP FLAT HOLE BBVA BBCONST BBEQ BBOP BVADD BVMUL
+%token NOT XOR ITE EQ LT LEQ GT GEQ PLUS MINUS MULT OPP LET DIST BBT BITOF BVAND BVOR BVXOR BVADD BVMUL
+%token INPU DEEP TRUE FALS ANDP ANDN ORP ORN XORP1 XORP2 XORN1 XORN2 IMPP IMPN1 IMPN2 EQUP1 EQUP2 EQUN1 EQUN2 ITEP1 ITEP2 ITEN1 ITEN2 EQRE EQTR EQCO EQCP DLGE LAGE LATA DLDE LADE FINS EINS SKEA SKAA QNTS QNTM RESO WEAK AND NOR OR NAND XOR1 XOR2 NXOR1 NXOR2 IMP NIMP1 NIMP2 EQU1 EQU2 NEQU1 NEQU2 ITE1 ITE2 NITE1 NITE2 TPAL TLAP TPLE TPNE TPDE TPSA TPIE TPMA TPBR TPBE TPSC TPPP TPQT TPQS TPSK SUBP FLAT HOLE BBVA BBCONST BBEQ BBOP BBADD BBMUL
 %token <int> INT SHARPINT
 %token <Big_int.big_int> BIGINT
 %token <string> VAR BINDVAR BITV
@@ -142,8 +142,8 @@ typ:
   | BBCONST                                                { Bbconst }
   | BBEQ                                                   { Bbeq  }
   | BBOP                                                   { Bbop  }
-  | BVADD                                                  { Bbadd }
-  | BVMUL                                                  { Bbmul }
+  | BBADD                                                  { Bbadd }
+  | BBMUL                                                  { Bbmul }
 ;
 
 clause:
@@ -190,6 +190,7 @@ term:   /* returns a SmtAtom.Form.pform or a SmtAtom.hatom */
   /* Atoms */
   | INT                                                    { Atom (Atom.hatom_Z_of_int ra $1) }
   | BIGINT                                                 { Atom (Atom.hatom_Z_of_bigint ra $1) }
+  | BITV                                                   { Atom (Atom.mk_bvconst ra (parse_bv $1)) }
   | LT name_term name_term                                 { match $2,$3 with |Atom h1, Atom h2 -> Atom (Atom.mk_lt ra h1 h2) | _,_ -> assert false }
   | LEQ name_term name_term                                { match $2,$3 with |Atom h1, Atom h2 -> Atom (Atom.mk_le ra h1 h2) | _,_ -> assert false }
   | GT name_term name_term                                 { match $2,$3 with |Atom h1, Atom h2 -> Atom (Atom.mk_gt ra h1 h2) | _,_ -> assert false }
@@ -200,9 +201,48 @@ term:   /* returns a SmtAtom.Form.pform or a SmtAtom.hatom */
   | MINUS name_term                                        { match $2 with | Atom h -> Atom (Atom.mk_opp ra h) | _ -> assert false }
   | OPP name_term                                          { match $2 with | Atom h -> Atom (Atom.mk_opp ra h) | _ -> assert false }
   | DIST args                                              { let a = Array.of_list $2 in Atom (Atom.mk_distinct ra (Atom.type_of a.(0)) a) }
-  | BITOF INT name_term                                    { match $3 with |Atom h -> (match Atom.type_of h with | TBV s -> Atom (Atom.mk_bitof ra s $2 h) | _ -> assert false) | _ -> assert false }
-  | BVAND name_term name_term                              { match $2,$3 with |Atom h1, Atom h2 -> (match Atom.type_of h1 with | TBV s -> Atom (Atom.mk_bvand ra s h1 h2) | _ -> assert false) | _,_ -> assert false }
-  | BVOR name_term name_term                               { match $2,$3 with |Atom h1, Atom h2 -> (match Atom.type_of h1 with | TBV s -> Atom (Atom.mk_bvor ra s h1 h2) | _ -> assert false) | _,_ -> assert false }
+  | BITOF INT name_term
+    { match $3 with
+      | Atom h -> (match Atom.type_of h with
+                   | TBV s -> Atom (Atom.mk_bitof ra s $2 h)
+                   | _ -> assert false)
+      | _ -> assert false }
+    
+  | BVAND name_term name_term
+    { match $2,$3 with
+      | Atom h1, Atom h2 -> (match Atom.type_of h1 with
+                             | TBV s -> Atom (Atom.mk_bvand ra s h1 h2)
+                             | _ -> assert false)
+      | _,_ -> assert false }
+    
+  | BVOR name_term name_term {
+    match $2,$3 with
+      | Atom h1, Atom h2 -> (match Atom.type_of h1 with
+                             | TBV s -> Atom (Atom.mk_bvor ra s h1 h2)
+                             | _ -> assert false)
+      | _,_ -> assert false
+    }
+  | BVXOR name_term name_term {
+    match $2,$3 with
+      | Atom h1, Atom h2 -> (match Atom.type_of h1 with
+                             | TBV s -> Atom (Atom.mk_bvxor ra s h1 h2)
+                             | _ -> assert false)
+      | _,_ -> assert false
+    }
+  | BVADD name_term name_term {
+    match $2,$3 with
+      | Atom h1, Atom h2 -> (match Atom.type_of h1 with
+                             | TBV s -> Atom (Atom.mk_bvadd ra s h1 h2)
+                             | _ -> assert false)
+      | _,_ -> assert false
+    }         
+  | BVMUL name_term name_term {
+    match $2,$3 with
+      | Atom h1, Atom h2 -> (match Atom.type_of h1 with
+                             | TBV s -> Atom (Atom.mk_bvmult ra s h1 h2)
+                             | _ -> assert false)
+      | _,_ -> assert false
+    }        
   | VAR                                                    { Atom (Atom.get ra (Aapp (get_fun $1, [||]))) }
   | VAR args                                               { Atom (Atom.get ra (Aapp (get_fun $1, Array.of_list $2))) }
 
